VmSemantics.v
@@ -1,0 +1,129 @@
+Require Import Term.
+Require Import Instr.
+
+Require Import List.
+Import ListNotations.
+
+Inductive vm_primR : Plc -> (Evidence*ev_stack) -> Instr -> (Evidence*ev_stack) -> Prop :=
+| vcopy : forall p ep, vm_primR p ep copy ep
+| vkmeas : forall i p q args e s,
+    let bs := invokeKIM i q args in
+    vm_primR p (e,s) (kmeas i q args) ((kk i args q p bs e),s)
+| vumeas : forall i p args e s,
+    let bs := invokeUSM i args in
+    vm_primR p (e,s) (umeas i args) ((uu i args p bs e),s)
+| vsign : forall p e s,
+    let bs := signEv e in
+    vm_primR p (e,s) sign ((gg p e bs),s)
+| vhash : forall p e s,
+    let bs := hashEv e in
+    vm_primR p (e,s) hash ((hh p bs),s)
+| vreqrpy : forall p e pTo pFrom s t,
+    vm_primR p (e,s) (reqrpy pFrom pTo t) (toRemote t pTo e,s)
+| vsplit : forall p sp1 sp2 e s,
+    let e1 := splitEv sp1 e in
+    let e2 := splitEv sp2 e in
+    vm_primR p (e,s) (Instr.split sp1 sp2) (e1, push_stack e2 s)
+(*| vbesr : forall p e s,
+    let (er,s') := pop_stack s in
+    let s'' := push_stack e s' in
+    (vm_primR p (e,s) besr (er,s'')).*)
+| vbesr : forall p e s,
+    vm_primR p (e,s) besr ((fst(pop_stack s)), (push_stack e (snd(pop_stack s))))
+| vjoins : forall p e (s:ev_stack),
+    (*let (er,s') := pop_stack s in
+    vm_primR p (e,s) joins (ss er e,s')*)
+    vm_primR p (e,s) joins (ss (fst(pop_stack s)) e,snd(pop_stack s))
+| vjoinp : forall p e (s:ev_stack),
+    vm_primR p (e,s) joinp (pp e (fst(pop_stack s)), snd(pop_stack s))
+| vbep : forall p e s evs1 evs2,
+    let res1 := parallel_att_vm_thread evs1 e in
+    let res2 := parallel_att_vm_thread evs2 (fst(pop_stack s)) in
+    vm_primR p (e,s) (bep evs1 evs2) (res1, push_stack res2 (snd(pop_stack s))).
+
+Lemma vm_primR_implies_vm_prim : forall p i ep1 ep2,
+    vm_primR p ep1 i ep2 -> vm_prim p ep1 i = ep2.
+Proof.
+  intros.
+  induction H; try (destruct ep); try (destruct s); reflexivity.
+Defined.
+
+Lemma vm_prim_implies_vm_primR : forall p i ep1 ep2,
+    vm_prim p ep1 i = ep2 -> vm_primR p ep1 i ep2.
+Proof.
+Admitted.
+
+Lemma vm_prim_iff_vm_primR : forall p i ep1 ep2,
+    vm_prim p ep1 i = ep2 <-> vm_primR p ep1 i ep2.
+Proof.
+  intros.
+  split.
+  - apply vm_prim_implies_vm_primR.
+  - apply vm_primR_implies_vm_prim.
+Defined.
+
+    
+
+
+
+Inductive att_vm'R : Plc -> (list Instr) -> (list Instr) -> (Evidence*ev_stack) -> (Evidence*ev_stack) -> Prop :=
+| att_vm'R_nil : forall p ep,
+    att_vm'R p [] [] ep ep
+| att_vm'R_step : forall p i is ep ep',
+    vm_primR p ep i ep' ->
+    att_vm'R p (i::is) is ep ep'
+| att_vm'R_trans : forall p is is' is'' ep ep' ep'',
+    att_vm'R p is is' ep ep' ->
+    att_vm'R p is' is'' ep' ep'' ->
+    att_vm'R p is is'' ep ep''.
+
+Definition att_vmR (p:Plc) (is:list Instr) (e:Evidence) (e':Evidence) : Prop :=
+  att_vm'R p is [] (e,[]) (e',[]).
+
+Require Import Coq.Program.Equality.
+Set Nested Proofs Allowed.
+
+Lemma pairf{A B:Type} : forall (p:A*B) e' v,
+    p = (e', v) -> fst p = e'.
+Proof.
+  intros.
+  subst. simpl. reflexivity.
+Defined.
+
+Lemma asdf : forall p e i e',
+    vm_primR p (e, []) i (e', []) -> fst (vm_prim p (e, []) i) = e'.
+Proof.
+  intros.
+  Check vm_prim_iff_vm_primR.
+  rewrite <- vm_prim_iff_vm_primR in H.
+  eapply pairf. eassumption.
+Defined.
+
+Lemma fdsa : forall p is is' e ep' e',
+    att_vm'R p is is' (e, []) ep' -> 
+    att_vm'R p is' [] ep' (e', []) ->
+    fst (att_vm' is p (e, [])) = e'.
+Proof.
+Admitted.
+
+Theorem att_vmR_implies_att_vm : forall p e e' is,
+    att_vmR p is e e' -> att_vm is p e = e'.
+Proof.
+  intros.
+  inversion H.
+  - cbv. reflexivity.
+  - unfold att_vm. unfold att_vm'. unfold fold_left.
+    apply asdf; assumption.
+    
+  - unfold att_vm.
+    subst.
+    eapply fdsa; eassumption.
+Defined.
+
+    
+    
+    
+  
+      
+    
+  
